Lampe/Tests/NewTest.lean
@@ -10,11 +10,155 @@ nr_def aaa<>(x : u8, n : u8) -> u8 {
     a
 }
 
+nr_def «asdf»<>() -> [u8; 5] {
+    let mut x = [0 : u8 ; 5];
+    for i in 0 : u8 .. 5 : u8 {
+            x[#cast(i) : u32] = #uAdd(i, 7 : u8) : u8;
+    }
+    ;
+    x;
+}
+
+#check Tp.denote
+
+lemma SLP.pure_star_iff_and [LawfulHeap α] {H : SLP α} : (⟦P⟧ ⋆ H) st ↔ P ∧ H st := by
+  simp [SLP.star, SLP.lift]
+  apply Iff.intro
+  · rintro ⟨st₁, st₂, hdis, hst, ⟨hp, rfl⟩, hH⟩
+    simp only [LawfulHeap.empty_union] at hst
+    cases hst
+    simp_all
+  · intro ⟨hP, hH⟩
+    exists ∅, st
+    simp_all
+
+lemma STHoare.pure_left_of_imp (h : P → STHoare lp Γ ⟦P⟧ E Q): STHoare lp Γ ⟦P⟧ E Q := by
+  simp_all [STHoare, THoare, SLP.pure_star_iff_and]
+
+-- lemma STHoare.exists_left_of_imp (h : P → STHoare lp Γ ⟦P⟧ E Q)
+--     : STHoare lp Γ (SLP.exists' fun h => ⟦P⟧) E Q := by
+--   sorry
+
+lemma STHoare.pure_left {E : Expr (Tp.denote lp) tp} {Γ P Q} : (P → STHoare lp Γ ⟦True⟧ E Q) → STHoare lp Γ ⟦P⟧ E Q := by
+  intro h
+  apply STHoare.pure_left_of_imp
+  intro
+  apply STHoare.consequence (h_hoare := h (by assumption))
+  · simp [SLP.lift, SLP.entails]
+  · intro; apply SLP.entails_self
+
+lemma STHoare.pure_left_nontriv {E : Expr (Tp.denote lp) tp} {Γ P Q}
+    : (P → STHoare lp Γ H E Q) → STHoare lp Γ (⟦P⟧ ⋆ H) E Q := by
+  intro h
+  simp_all only [STHoare, THoare, SLP.star_assoc, SLP.pure_star_iff_and, implies_true]
+
+
+def loopInvAux (u : U 8) : List.Vector (U 8) 5 :=
+  let asdf := List.range' 7 u.toNat |>.take 5 |>.map (BitVec.ofNat 8 ·)
+  let asdf2 : List (U 8) := asdf ++ (List.replicate (5 - asdf.length) 0)
+  have : asdf2.length = 5 := by
+    simp [asdf2, asdf]
+  ⟨asdf2, this⟩
+
+theorem loopInvAux_induction :
+    (loopInvAux x).set x.toNat (x + 7#8) = loopInvAux (x + 1#8) := by
+  sorry
+
+
+-- theorem loopInvAux_induction2 :
+--   List.Vector.eraseIdx 0 ((loopInvAux 0).insertIdx 1 1) =
+--   loopInvAux 1 := by
+--   unfold loopInvAux
+--   ext i t
+--   fin_cases i <;> simp <;> rfl
+
+open STHoare
+example : STHoare p Γ ⟦⟧ (asdf.fn.body _ h![] |>.body h![]) fun
+    v => v = ⟨[7, 8, 9, 10, 11], by simp⟩ := by
+  simp only [asdf]
+
+  apply letIn_intro
+  apply litU_intro
+  intro v; apply pure_left; rintro rfl
+
+  apply letIn_intro
+  apply mkArray_intro
+  simp
+
+  intro v;
+  apply pure_left; simp; rintro rfl
+
+  apply letIn_intro
+  apply ref_intro'
+  intro v; simp
+
+  apply letIn_intro
+  apply consequence_frame_left; apply litU_intro
+  simp; exact SLP.entails_self
+  intro v; apply pure_left_nontriv; rintro rfl
+
+  apply letIn_intro
+  apply consequence_frame_left litU_intro
+  simp; exact SLP.entails_self
+  intro v; apply pure_left_nontriv; rintro rfl
+
+  apply letIn_intro
+  apply STHoare.consequence_frame_left (STHoare.loop_inv_intro
+      (fun u _ _ => [v ↦ ⟨Tp.array (Tp.u 8) 5, loopInvAux u⟩])
+      (fun x hlo hhi => ?_))
+  · simp
+    sl
+    change 0 ≤ 5
+    decide
+  · simp
+    apply letIn_intro
+    apply consequence_frame_left litU_intro
+    · simp; exact SLP.entails_self
+    intro v; apply pure_left_nontriv; rintro rfl
+
+    apply letIn_intro
+    apply consequence_frame_left uAdd_intro
+    · simp; exact SLP.entails_self
+    intro v; apply pure_left_nontriv; simp; intro h; rintro rfl
+
+    apply letIn_intro
+    apply consequence_frame_left cast_intro
+    simp; exact SLP.entails_self
+    intro vv
+
+    apply letIn_intro
+    apply consequence_frame_left modifyLens_intro
+    nth_rewrite 1 [SLP.star_comm]
+    exact SLP.entails_self
+    intro vvv
+
+    apply ramified_frame_top var_intro
+    simp
+    sl
+    congr
+    simp [Access.modify]
+    simp [Builtin.replaceArray']
+    ext x
+    fin_cases x <;> congr <;> sorry
+
+  intro unt; apply letIn_intro
+  apply consequence_frame_left readRef_intro
+  simp; sl
+  intro v; simp; apply pure_left_nontriv; rintro rfl
+  rw [SLP.star_comm]
+  apply pure_left_nontriv; intro h -- h is a weird hypothesis that isn't necessary
+
+  apply ramified_frame_top var_intro
+  sl
+  simp_all
+  rfl
+
 def addOne (u : U 8) : U 8 := u + 1
 
-def asdf (n : Nat) := Nat.repeat addOne n
+def asdff (n : Nat) := Nat.repeat addOne n
 
-def thm : Nat.repeat addOne n u = u + n := by sorry
+def thm : Nat.repeat addOne n u = u + n := by
+  sorry
 
 example (h : x < 100) (hn : n < 100)
     : STHoare p Γ ⟦⟧ (aaa.fn.body _ h![] |>.body h![x, n]) fun v => v = x + n := by
